Weidenbach_Book/Propo_CDCL_Termination.thy
@@ -2,6 +2,7 @@ theory Propo_CDCL_Termination
 imports Propo_CDCL
 begin
 
+text \<open>The condition that no learned clause is a tautology is overkill (in the sense that the no-duplicate condition is enough), but we can reuse @{term build_all_simple_clss}.\<close>
 definition cdcl_all_inv_mes where
   "cdcl_all_inv_mes S =
     (no_strange_atm S \<and> cdcl_M_level_inv S \<and>  finite (atms_of_m (clauses S))
